double_anno_inter/coq/syntax_algo_int_and_arrow.v
@@ -1,0 +1,537 @@
+
+(*
+Update started on February 12, 2021
+*)
+
+(*
+This file contains the updates suggested by Bruno.
+
+Algorithmic disjointness definition:
+
+A *a B = not (Int & (Top -> Bot) <: A & B)
+
+*)
+
+Require Import TLC.LibLN.
+Require Import Program.Equality.
+
+(* Require Import LibTactics. *)
+(*Implicit Types x : var.*)
+(** syntax *)
+
+Inductive typ : Set :=  (*r type *)
+ | typ_top : typ
+ | t_int : typ
+ | t_bot : typ
+ | t_arrow : typ -> typ -> typ
+ | t_union : typ -> typ -> typ
+ | t_and : typ -> typ -> typ.
+
+Inductive exp : Set :=  (*r expression *)
+ | e_var_b  : nat -> exp
+ | e_var_f  : var -> exp
+ | e_lit    : nat -> exp
+ | e_ann    : exp -> typ -> exp
+ | e_abs    : exp -> exp
+ | e_app    : exp -> exp -> exp
+ | e_typeof : exp -> typ -> exp -> typ -> exp -> exp.
+
+Inductive dirflag : Set :=  (*r typing direction *)
+ | infer : dirflag
+ | check : dirflag.
+
+(** Binding are mapping to term variables.
+ [x ~: T] is a typing assumption *)
+
+ Inductive bind : Set :=
+ | bind_typ : typ -> bind.
+
+Notation "x ~: T" := (x ~ T)
+ (at level 23, left associativity) : env_scope.
+
+(** Environment is an associative list of bindings. *)
+
+
+ Definition env := LibEnv.env typ.
+
+Inductive okt : env -> Prop :=
+| okt_empty :
+     okt empty
+| okt_typ : forall E x T,
+     okt E-> x # E -> okt (E & x ~: T).
+
+
+(* EXPERIMENTAL *)
+(** auxiliary functions on the new list types *)
+(** library functions *)
+(** subrules *)
+(** arities *)
+(** opening up abstractions *)
+Fixpoint open_exp_wrt_exp_rec (k:nat) (e_5:exp) (e__6:exp) {struct e__6}: exp :=
+  match e__6 with
+  | (e_var_b nat) => If (k = nat) then e_5 else (e_var_b nat)
+  | (e_var_f x) => e_var_f x
+  | (e_lit i5) => e_lit i5
+  | (e_ann e A) => e_ann (open_exp_wrt_exp_rec k e_5 e) A
+  | (e_abs e) => e_abs (open_exp_wrt_exp_rec (S k) e_5 e)
+  | (e_app e1 e2) => e_app (open_exp_wrt_exp_rec k e_5 e1) (open_exp_wrt_exp_rec k e_5 e2)
+  | (e_typeof e A e1 B e2) => e_typeof (open_exp_wrt_exp_rec k e_5 e) A (open_exp_wrt_exp_rec (S k) e_5 e1) B (open_exp_wrt_exp_rec (S k) e_5 e2)
+end.
+
+Definition open_exp_wrt_exp e_5 e__6 := open_exp_wrt_exp_rec 0 e__6 e_5.
+
+(** Notation for opening up binders with type or term variables *)
+
+Notation "t 'open_ee_var' x" := (open_exp_wrt_exp t (e_var_f x)) (at level 67).
+
+
+(** terms are locally-closed pre-terms *)
+(** definitions *)
+
+(* defns LC_exp *)
+Inductive lc_exp : exp -> Prop :=    (* defn lc_exp *)
+ | lc_e_var_f : forall (x:var),
+     (lc_exp (e_var_f x))
+ | lc_e_lit : forall i5,
+     (lc_exp (e_lit i5))
+ | lc_e_ann : forall (e:exp) (A:typ),
+     (lc_exp e) ->
+     (lc_exp (e_ann e A))
+ | lc_e_abs : forall (L:vars) (e:exp),
+      ( forall x , x \notin  L  -> lc_exp  ( open_exp_wrt_exp e (e_var_f x) )  )  ->
+     (lc_exp (e_abs e))
+ | lc_e_app : forall (e1 e2:exp),
+     (lc_exp e1) ->
+     (lc_exp e2) ->
+     (lc_exp (e_app e1 e2))
+ | lc_e_typeof : forall (L:vars) (e:exp) (A:typ) (e1:exp) (B:typ) (e2:exp),
+     (lc_exp e) ->
+     ( forall x , x \notin  L  -> lc_exp  ( open_exp_wrt_exp e1 (e_var_f x) )  ) ->
+     ( forall x , x \notin  L  -> lc_exp  ( open_exp_wrt_exp e2 (e_var_f x) )  ) ->
+     (lc_exp (e_typeof e A e1 B e2)).
+(** free variables *)
+Fixpoint fv_exp (e_5:exp) : vars :=
+  match e_5 with
+  | (e_var_b nat) => \{}
+  | (e_var_f x) => \{x}
+  | (e_lit i5) => \{}
+  | (e_ann e A) => (fv_exp e)
+  | (e_abs e) => (fv_exp e)
+  | (e_app e1 e2) => (fv_exp e1) \u (fv_exp e2)
+  | (e_typeof e A e1 B e2) => (fv_exp e) \u (fv_exp e1) \u (fv_exp e2)
+end.
+
+(** substitutions *)
+Fixpoint subst_exp (e_5:exp) (x5:var) (e__6:exp) {struct e__6} : exp :=
+  match e__6 with
+  | (e_var_b nat) => e_var_b nat
+  | (e_var_f x) => (If x = x5 then e_5 else (e_var_f x))
+  | (e_lit i5) => e_lit i5
+  | (e_ann e A) => e_ann (subst_exp e_5 x5 e) A
+  | (e_abs e) => e_abs (subst_exp e_5 x5 e)
+  | (e_app e1 e2) => e_app (subst_exp e_5 x5 e1) (subst_exp e_5 x5 e2)
+  | (e_typeof e A e1 B e2) => e_typeof (subst_exp e_5 x5 e) A (subst_exp e_5 x5 e1) B (subst_exp e_5 x5 e2)
+end.
+
+
+(** definitions *)
+
+(* defns PreValue *)
+Inductive pexpr : exp -> Prop :=    (* defn pexpr *)
+ | pexpr_int : forall i5,
+     pexpr (e_lit i5)
+ | pexpr_abs : forall (e:exp) (A B:typ),
+     lc_exp (e_abs e) ->
+     pexpr (e_ann  ( (e_abs e) )  (t_arrow A B)).
+
+(* defns RExpr *)
+Inductive rexpr : exp -> Prop :=    (* defn rexpr *)
+ | rexpr_app : forall (e1 e2:exp),
+     lc_exp e1 ->
+     lc_exp e2 ->
+     rexpr  ( (e_app e1 e2) )
+ | rexpr_typeof : forall (e:exp) (A:typ) (e1:exp) (B:typ) (e2:exp),
+     lc_exp e ->
+     lc_exp e1 ->
+     lc_exp e2 ->
+     rexpr (e_typeof e A e1 B e2).
+
+(* defns Value *)
+Inductive value : exp -> Prop :=    (* defn value *)
+ | value_val : forall (p:exp) (A:typ),
+     pexpr p ->
+     value (e_ann p A).
+
+(* defns UExpr *)
+Inductive uexpr : exp -> Prop :=    (* defn uexpr *)
+ | uexpr_rexpr : forall (r:exp),
+     rexpr r ->
+     uexpr r
+ | uexpr_pexpr : forall (p:exp),
+     pexpr p ->
+     uexpr p
+ | uexpr_anno : forall (u:exp) (A:typ),
+     uexpr u ->
+     uexpr (e_ann u A).
+
+(* defns FindType *)
+Inductive findtype : exp -> typ -> Prop :=    (* defn findtype *)
+ | findtype_int : forall i5,
+     findtype (e_lit i5) t_int
+ | findtype_arrow : forall (e:exp) (A B:typ),
+     lc_exp (e_abs e) ->
+     findtype  ( (e_ann  ( (e_abs e) )  (t_arrow A B)) )   (t_arrow A B).
+
+
+(* defns Subtyping *)
+Reserved Notation "A <: B" (at level 80).
+Inductive subtyping : typ -> typ -> Prop :=    (* defn subtyping *)
+ | s_top : forall A, A <: typ_top
+ | s_btm : forall (A:typ),
+     t_bot <: A
+ | s_int :
+     subtyping t_int t_int
+ | s_arrow : forall (A1 A2 B1 B2:typ),
+     B1 <: A1 ->
+     A2 <: B2 ->
+     (t_arrow A1 A2) <: (t_arrow B1 B2)
+ | s_ora : forall (A1 A2 A:typ),
+     A1 <: A ->
+     A2 <: A ->
+     (t_union A1 A2) <: A
+ | s_orb : forall (A A1 A2:typ),
+     A <: A1 ->
+     A <: (t_union A1 A2)
+ | s_orc : forall (A A1 A2:typ),
+     A <: A2 ->
+     A <: (t_union A1 A2)
+ | s_anda : forall A A1 A2,
+     A <: A1 ->
+     A <: A2 ->
+     A <: (t_and A1 A2)
+ | s_andb : forall A1 A2 A,
+     A1 <: A ->
+     (t_and A1 A2) <: A
+ | s_andc : forall A1 A2 A,
+     A2 <: A ->
+     (t_and A1 A2) <: A
+where "A <: B" := (subtyping A B) : env_scope.
+
+Hint Constructors pexpr rexpr value uexpr findtype subtyping lc_exp ok okt.
+
+(**********************************)
+(*****  Subtyping Properties  *****)
+(**********************************)
+
+Lemma sub_or : forall A B C, (t_union A B) <: C -> A <: C /\ B <: C.
+Proof.
+intros; inductions H; try solve [split*].
+specialize (IHsubtyping A B).
+forwards* : IHsubtyping.
+specialize (IHsubtyping A B).
+forwards* : IHsubtyping.
+specialize (IHsubtyping1 A B).
+specialize (IHsubtyping2 A B).
+forwards*: IHsubtyping1.
+Defined.
+
+Lemma sub_and : forall A B C, A <: (t_and B C) -> A <: B /\ A <: C.
+Proof.
+intros; inductions H; try solve [split*].
+specialize (IHsubtyping1 B C).
+specialize (IHsubtyping2 B C).
+forwards*: IHsubtyping1.
+specialize (IHsubtyping B C).
+forwards*: IHsubtyping.
+specialize (IHsubtyping B C).
+forwards*: IHsubtyping.
+Defined.
+
+Lemma sub_refl : forall A, A <: A.
+  induction A; eauto.
+Defined.
+
+Hint Resolve sub_refl.
+
+
+Lemma sub_transitivity : forall B A C, A <: B -> B <: C -> A <: C.
+Proof.
+induction B; intros;
+generalize H0 H; clear H0; clear H; generalize A; clear A.
+- intros; inductions H0; eauto. 
+- intros; inductions H; eauto.
+- intros; inductions H; eauto.
+- induction C; intros; inverts* H0.
+  induction A; inverts* H.
+- intros. apply sub_or in H0. destruct H0.
+  inductions H; eauto.
+- intros. apply sub_and in H. destruct H.
+  inductions H0; eauto.
+Defined.
+
+
+(*************************)
+(***** Ordinary Types ****)
+(*************************)
+
+Inductive Ord : typ -> Prop :=
+| o_top : Ord typ_top
+| o_int : Ord t_int
+| o_arrow : forall t1 t2, Ord (t_arrow t1 t2).
+(*| o_union : forall t1 t2, Ord t1 -> Ord t2 -> Ord (t_union t1 t2).*)
+
+
+(****************************************)
+(**********  Dijoint Specs    ***********)
+(****************************************)
+
+Definition DisjSpec A B := forall C, Ord C -> not (C <:  (t_and A B)).
+Notation "A *s B" := (DisjSpec A B) (at level 80).
+
+(****************************************)
+(***********  Dijoint Algo   ************)
+(****************************************)
+
+Definition DisjAlgo A B := 
+    not ((t_and t_int (t_arrow typ_top t_bot)) <: (t_and A B)).
+Notation "A *a B" := (DisjAlgo A B) (at level 80).
+
+(**********************************)
+(****  DisjSpec Properties  ****)
+(**********************************)
+
+Lemma ord_sub_bot_false : forall A, Ord A -> A <: t_bot -> False.
+Proof.
+  intros.
+  dependent induction H; inversion H0.
+Defined.
+
+Lemma not_sub_and : forall A1 A2, forall A, Ord A ->
+not (A <: (t_and A1 A2)) -> not((A <: A1) /\ (A <: A2)).
+Proof.
+  intros.
+  unfold not in *. intros.
+  apply H0; destruct~ H1.
+Defined.
+
+Lemma ord_sub_and_or : forall B C, forall A, Ord A ->
+not (A <: (t_and B C)) -> not(A <: B) \/ not(A <: C) \/ not (A <: (t_and B C)).
+Proof.
+  intros.
+  unfold not in *. auto.
+Defined.
+
+Lemma not_sub_or_inv : forall A A1 A2, Ord A -> not (A <: A1) -> not (A <: A2) -> not (A <: (t_union A1 A2)).
+Proof.
+  intros.
+  unfold not in *.
+  intros. inductions H; inverts* H2.
+Defined.
+
+Lemma btm_sub : forall A, t_bot <: A.
+Proof.
+  intros; auto.
+Defined.
+
+Lemma ord_sub_union : forall A, Ord A -> forall A1 A2, A <: t_union A1 A2 -> A <: A1 \/ A <: A2.
+Proof.
+  intros A H.
+  dependent induction H; intros.
+  inverts* H.
+  inverts* H.
+  inverts* H.
+Defined.
+
+Lemma not_sub_and1_inv : forall A A1 A2, Ord A -> not (A <: A1) -> not (A <: (t_and A1 A2)).
+Proof.
+  intros.
+  unfold not in *.
+  intros. inductions H; inverts* H1.
+Defined.
+
+Lemma not_sub_and2_inv : forall A A1 A2, Ord A -> not (A <: A2) -> not (A <: (t_and A1 A2)).
+Proof.
+  intros.
+  unfold not in *.
+  intros. inductions H; inverts* H1.
+Defined.
+
+Lemma disj_sub_union : forall A B C, A *s C -> B *s C -> t_union A B *s C.
+Proof.
+  intros.
+  unfold DisjSpec in *. intros.
+  unfold not in *. intros.
+  specialize (H C0).
+  apply H; auto.
+  apply sub_and in H2.
+  destruct H2.
+  lets: ord_sub_union C0 H1 A B H2.
+  destruct H4.
+  apply s_anda; auto.
+  specialize (H0 C0).
+  forwards*: H0.
+Defined.
+
+Lemma disj_spec_union : forall A B C, t_union A B *s C -> A *s C /\ B *s C.
+Proof.
+  unfold DisjSpec; unfold not; intros.
+  split.
+  - intros. apply sub_and in H1. destruct H1.
+    specialize (H C0).
+    apply H; auto.
+  - intros. apply sub_and in H1. destruct H1.
+    specialize (H C0).
+    apply H; auto.
+Defined.
+
+Lemma disj_spec_union1 : forall A B C, A *s t_union B C -> A *s B /\ A *s C.
+Proof.
+  unfold DisjSpec; unfold not; intros.
+  split.
+  - intros. apply sub_and in H1. destruct H1.
+    specialize (H C0).
+    apply H; auto.
+  - intros. apply sub_and in H1. destruct H1.
+    specialize (H C0).
+    apply H; auto.
+Defined.
+
+Lemma ord_sub_disj_spec_false : forall A, Ord A -> 
+forall B C, B *s C -> A <: (t_and B C) -> False.
+Proof.
+ unfold DisjSpec; unfold not; intros.
+ apply sub_and in H1. destruct H1.
+ specialize (H0 A).
+ forwards*: H0 H.
+Defined.
+
+Lemma Disj_sym_spec : forall A B, A *s B -> B *s A.
+Proof.
+  unfold DisjSpec; unfold not; intros.
+  intros.
+  forwards*: H H0.
+  apply sub_and in H1. destruct H1.
+  apply s_anda; auto.
+Defined.    
+
+Lemma Disj_soundness : forall A B, A *a B -> A *s B.
+Proof.
+(* Disj_soundness Soundness Proof *)
+  intros; unfold DisjAlgo in H; unfold not in H.
+  unfold DisjSpec; unfold not; intros; apply H.
+  apply sub_and in H1; destruct H1.
+  dependent induction H0; auto.
+ - assert (t_int <: typ_top); auto.
+   eapply sub_transitivity in H1; eauto.
+   eapply sub_transitivity in H2; eauto.
+ - assert ((t_arrow typ_top t_bot) <: (t_arrow t1 t2)); auto.
+   eapply sub_transitivity in H1; eauto.
+   eapply sub_transitivity in H2; eauto.
+Qed.
+
+Lemma Disj_completeness : forall A B,  A *s B -> A *a B.
+Proof.
+   intros A. inductions A.
+  - unfold DisjAlgo. unfold not. intros.
+    apply sub_and in H0. destruct H0.
+    inductions B.
+    admit.
+    admit.
+    inverts* H1. inversion H5. inversion H5.
+    admit.
+    admit.
+    inverts* H1. admit. admit. admit.
+  - admit.
+  - unfold DisjAlgo. unfold not. intros.
+    inverts* H0. inverts* H4. inversion H3. inversion H3.
+    inverts* H4. inversion H3. inverts* H4. inversion H3.
+  - admit.
+  - admit.
+  - unfold DisjAlgo. unfold not. intros.
+    inverts* H0.
+    inverts* H4.
+    unfold DisjSpec in H. unfold not in H.
+Admitted.
+
+(* defns Typing *)
+Inductive typing : env -> exp -> dirflag -> typ -> Prop :=    (* defn typing *)
+ | typ_lit : forall (G:env) i5,
+      okt  G  ->
+     typing G (e_lit i5) infer t_int
+ | typ_var : forall (G:env) (x:var) (A:typ),
+      okt  G  ->
+      binds  x A G  ->
+     typing G (e_var_f x) infer A
+ | typ_ann : forall (G:env) (e:exp) (A:typ),
+     typing G e check A ->
+     typing G (e_ann e A) infer A
+ | typ_app : forall (G:env) (e1 e2:exp) (B A:typ),
+     typing G e1 infer (t_arrow A B) ->
+     typing G e2 check A ->
+     typing G (e_app e1 e2) infer B
+ | typ_sub : forall (G:env) (e:exp) (A B:typ),
+     typing G e infer B ->
+     subtyping B A ->
+     typing G e check A
+ | typ_abs : forall (L:vars) (G:env) (e:exp) (A B:typ),
+      ( forall x , x \notin  L  -> typing  (G & x ~: A )   ( open_exp_wrt_exp e (e_var_f x) )  check B )  ->
+     typing G (e_abs e) check (t_arrow A B)
+ | typ_typeof : forall (L:vars) (G:env) (e:exp) (A:typ) (e1:exp) (B:typ) (e2:exp) (C:typ),
+     typing G e check (t_union A B) ->
+     ( forall x , x \notin  L  -> typing  (G & x ~: A )   ( open_exp_wrt_exp e1 (e_var_f x) )  check C ) ->
+     ( forall x , x \notin  L  -> typing  (G & x ~: B )   ( open_exp_wrt_exp e2 (e_var_f x) )  check C ) ->
+     A *s B ->
+     typing G (e_typeof e A e1 B e2) check C.
+
+Hint Constructors typing.
+
+(* defns Reduction *)
+Reserved Notation "e --> e'" (at level 80).
+Inductive step : exp -> exp -> Prop :=    (* defn step *)
+ | step_int : forall i5,
+     step (e_lit i5) (e_ann (e_lit i5) t_int)
+ | step_appl : forall (e1 e2 e1':exp),
+     lc_exp e2 ->
+     step e1 e1' ->
+     step (e_app e1 e2) (e_app e1' e2)
+ | step_appr : forall (v e e':exp),
+     value v ->
+     step e e' ->
+     step (e_app v e) (e_app v e')
+ | step_beta : forall (e:exp) (A1 B1 A2 B2:typ) (p:exp) (C:typ),
+     lc_exp (e_abs e) ->
+     pexpr p ->
+     (e_app  ( (e_ann (e_ann  ( (e_abs e) )  (t_arrow A1 B1)) (t_arrow A2 B2)) ) ( (e_ann p C) ) ) --> (e_ann (e_ann  (  (open_exp_wrt_exp  e (e_ann p A1) )  )  B1) B2)
+ | step_beta_abs : forall (e:exp) (A1 B1 A2 B2:typ) (p:exp) (C:typ) x,
+     lc_exp (e_abs e) ->
+     p = (e_abs x) ->
+     (e_app  ( (e_ann (e_ann  ( (e_abs e) )  (t_arrow A1 B1)) (t_arrow A2 B2)) ) ( p ) ) --> (e_ann (e_ann  (  (open_exp_wrt_exp  e (e_ann (e_ann p A2) A1) )  )  B1) B2)
+ | step_ann : forall (e:exp) (A:typ) (e':exp),
+      not ( value (e_ann e A) )  ->
+     step e e' ->
+     step (e_ann e A) (e_ann e' A)
+ | step_rm_ann : forall (p:exp) (A B:typ),
+     pexpr p ->
+     step (e_ann (e_ann p A) B) (e_ann p B)
+ | step_lam_ann : forall (e:exp) (A B:typ),
+     lc_exp (e_abs e) ->
+     step (e_ann  ( (e_abs e) )  (t_arrow A B)) (e_ann (e_ann  ( (e_abs e) )  (t_arrow A B)) (t_arrow A B))
+ | step_typeof : forall (e:exp) (A:typ) (e1:exp) (B:typ) (e2 e':exp),
+     lc_exp (e_typeof e A e1 B e2) ->
+     step e e' ->
+     step (e_typeof e A e1 B e2) (e_typeof e' A e1 B e2)
+ | step_typeofl : forall (p:exp) (A:typ) (e1:exp) (B:typ) (e2:exp) (x:var) (C:typ) (D:typ),
+     lc_exp (e_typeof (e_ann p D) A e1 B e2) ->
+     pexpr p ->
+     findtype p C ->
+     subtyping C A ->
+     step (e_typeof (e_ann p D) A e1 B e2)  (open_exp_wrt_exp e1 (e_ann p A) )
+ | step_typeofr : forall (p:exp) (A:typ) (e1:exp) (B:typ) (e2:exp) (x:var) (C:typ) (D:typ),
+    lc_exp (e_typeof (e_ann p D) A e1 B e2) ->
+     pexpr p ->
+     findtype p C ->
+     subtyping C B ->
+     step (e_typeof (e_ann p D) A e1 B e2)  (open_exp_wrt_exp  e2 (e_ann p B) )
+where "e --> e'" := (step e e') : env_scope.
+
+Hint Constructors step.
